tmp

arm/proofs/ldst.ml
@@ -25,7 +25,8 @@ let LD1_1_SIMD_64_IMM_POST_CORRECT = time prove
                C_ARGUMENTS [x] s /\
                read (memory :> bytes64 x) s = a)
           (\s. read PC s = word (pc + 0x04) /\
-               read Q0 s = (word_zx:int64->int128) a)
+               read Q0 s = (word_zx:int64->int128) a /\
+               read X0 s = word_add x (word 8))
           (MAYCHANGE [PC; X0],, MAYCHANGE [Q0])`,
   MAP_EVERY X_GEN_TAC [`x:int64`; `a:int64`; `pc:num`] THEN
   REWRITE_TAC[C_ARGUMENTS] THEN
@@ -36,8 +37,8 @@ let LD1_1_SIMD_64_IMM_POST_CORRECT = time prove
   );;
 
 (* ------------------------------------------------------------------------- *)
-(* ST1, one register, SIMD, 128-bit, immediate offset, post-index *)
-(* ST1 v0, [x0], #16 *)
+(* st1, one register, SIMD, 128-bit, immediate offset, post-index *)
+(* st1 v0, [x0], #16 *)
 let ST1_1_SIMD_128_IMM_POST = define_word_list "ST1_1_SIMD_128_IMM_POST"
   `[word 0x00; word 0x78; word 0x9F; word 0x4C]:byte list`;;
 
@@ -45,7 +46,7 @@ let ST1_1_SIMD_128_IMM_POST_EXEC = ARM_MK_EXEC_RULE ST1_1_SIMD_128_IMM_POST;;
 
 let ST1_1_SIMD_128_IMM_POST_CORRECT = time prove
  (`!x a pc.
-      nonoverlapping (word pc,0x04) (x,8 * 16)
+      nonoverlapping (word pc,0x04) (x,16)
       ==>
         ensures arm
              (\s. aligned_bytes_loaded s (word pc) ST1_1_SIMD_128_IMM_POST /\
@@ -53,7 +54,8 @@ let ST1_1_SIMD_128_IMM_POST_CORRECT = time prove
                   C_ARGUMENTS [x] s /\
                   read Q0 s = a)
              (\s. read PC s = word (pc + 0x04) /\
-                  read (memory :> bytes128 x) s = a)
+                  read (memory :> bytes128 x) s = a /\
+                  read X0 s = word_add x (word 16))
              (MAYCHANGE [PC; X0],,
               MAYCHANGE [memory :> bytes128 x])`,
   MAP_EVERY X_GEN_TAC [`x:int64`; `a:int128`; `pc:num`] THEN
@@ -66,3 +68,48 @@ let ST1_1_SIMD_128_IMM_POST_CORRECT = time prove
   );;
 
 (* ------------------------------------------------------------------------- *)
+(* ld2, two register, SIMD, 128-bit, immediate offset, post-index *)
+(* ld2 v0, [x0], #32 *)
+let LD2_SIMD_128_IMM_POST = define_word_list "LD2_SIMD_128_IMM_POST"
+  `[word 0x00; word 0x88; word 0xDF; word 0x4C]:byte list`;;
+
+let LD2_SIMD_128_IMM_POST_EXEC = ARM_MK_EXEC_RULE LD2_SIMD_128_IMM_POST;;
+
+
+let mc_length_th, decode_ths = LD2_SIMD_128_IMM_POST_EXEC;;
+
+let LD2_SIMD_128_IMM_POST_CORRECT = time prove
+ (`!x a b pc.
+     ensures arm
+          (\s. aligned_bytes_loaded s (word pc) LD2_SIMD_128_IMM_POST /\
+               read PC s = word pc /\
+               C_ARGUMENTS [x] s /\
+               read (memory :> bytes128 x) s = a /\
+               read (memory :> bytes128 (word_add x (word 0x80))) s = b)
+          (\s. read PC s = word (pc + 0x04) /\
+               read Q0 s = ((word_join:(96 word->32 word->128 word))
+                             ((word_join:(64 word->32 word->96 word))
+                               ((word_join:(32 word->32 word->64 word))
+                                 (word_subword a (0,32)) (word_subword a (64,32)))
+                                   (word_subword b (0,32))) (word_subword b (64,32))) /\
+               read Q1 s = ((word_join:(96 word->32 word->128 word))
+                             ((word_join:(64 word->32 word->96 word))
+                               ((word_join:(32 word->32 word->64 word))
+                                 (word_subword a (32,32)) (word_subword a (96,32)))
+                                   (word_subword b (32,32))) (word_subword b (96,32))) /\
+               read X0 s = word_add x (word 32))
+          (MAYCHANGE [PC; X0],, MAYCHANGE [Q0; Q1])`,
+  MAP_EVERY X_GEN_TAC [`x:int64`; `a:int128`; `b:int128`; `pc:num`] THEN
+  REWRITE_TAC[C_ARGUMENTS] THEN
+  ENSURES_INIT_TAC "s0" THEN
+  BIGNUM_DIGITIZE_TAC "a_" `read (memory :> bytes128 x) s0` THEN
+  BIGNUM_DIGITIZE_TAC "b_" `read (memory :> bytes128 (word_add x (word 128))) s0` THEN
+
+  ARM_ACCSTEPS_TAC LD2_SIMD_128_IMM_POST_EXEC [] [1] THEN
+  ARM_VERBOSE_STEP_TAC LD2_SIMD_128_IMM_POST_EXEC "S0" THEN
+  ARM_STEP_TAC LD2_SIMD_128_IMM_POST_EXEC [] "S0" THEN
+  ARM_BASIC_STEP_TAC decode_ths "s0"
+
+  ENSURES_FINAL_STATE_TAC THEN
+  ASM_REWRITE_TAC[]
+  );;
